revm: add support for more links for control instructions

CoqOfRust/core/num/links/mod.v
@@ -89,3 +89,44 @@ Module Impl_usize.
   Proof.
   Admitted.
 End Impl_usize.
+
+Module Impl_isize.
+  Import Impl_usize.
+
+  Definition Self : Set := Isize.t.
+
+  (* pub const MAX: Self *)
+  Instance run_max :
+    Run.Trait num.Impl_isize.value_MAX [] [] [] (Ref.t Pointer.Kind.Raw Self).
+  Proof.
+    constructor.
+    run_symbolic.
+  Defined.
+
+  (* pub const MIN: Self *)
+  Instance run_min :
+    Run.Trait num.Impl_isize.value_MIN [] [] [] (Ref.t Pointer.Kind.Raw Self).
+  Proof.
+    constructor.
+    run_symbolic.
+  Defined.
+
+  (* pub const fn saturating_add(self, rhs: Self) -> Self *)
+  Instance run_saturating_add (self rhs: Self) :
+    Run.Trait num.Impl_isize.saturating_add [] [] [ φ self; φ rhs ] Self.
+  Proof.
+    constructor.
+    run_symbolic.
+  Defined.
+
+  Instance run_saturating_mul (self rhs: Self) :
+    Run.Trait num.Impl_isize.saturating_mul [] [] [ φ self; φ rhs ] Self.
+  Proof.
+  Admitted.
+
+  (* pub const fn overflowing_sub(self, rhs: Self) -> (Self, bool) *)
+  Instance run_overflowing_sub (self rhs: Self) :
+    Run.Trait num.Impl_isize.overflowing_sub [] [] [ φ self; φ rhs ] (Self * bool).
+  Proof.
+  Admitted.
+End Impl_isize.
