CoqOfRust/core/links/error.v
@@ -1,0 +1,53 @@
+Require Import CoqOfRust.CoqOfRust.
+Require Import CoqOfRust.links.M.
+
+(* pub struct Request<'a>(Tagged<dyn Erased<'a> + 'a>); *)
+Module Request.
+  Parameter t : Set.
+
+  Parameter to_value : t -> Value.t.
+
+  Global Instance IsLink : Link t := {
+    Φ := Ty.path "core::error::Request";
+    φ := to_value;
+  }.
+
+  Definition of_ty : OfTy.t (Ty.path "core::error::Request").
+  Proof. eapply OfTy.Make with (A := t); reflexivity. Defined.
+  Smpl Add apply of_ty : of_ty.
+End Request.
+
+(*
+pub trait Error: Debug + Display {
+    // Provided methods
+    fn source(&self) -> Option<&(dyn Error + 'static)> { ... }
+    fn description(&self) -> &str { ... }
+    fn cause(&self) -> Option<&dyn Error> { ... }
+    fn provide<'a>(&'a self, request: &mut Request<'a>) { ... }
+}
+*)
+Module Error.
+  Definition trait (Self : Set) `{Link Self} : TraitMethod.Header.t :=
+    ("core::error::Error", [], [], Φ Self).
+
+  Definition Run_description (Self : Set) `{Link Self} : Set :=
+    TraitMethod.C (trait Self) "description" (fun method =>
+      forall (self : Ref.t Pointer.Kind.Ref Self),
+      Run.Trait method [] [] [ φ self ] (Ref.t Pointer.Kind.Ref string)
+    ).
+
+  Definition Run_provide (Self : Set) `{Link Self} : Set :=
+    TraitMethod.C (trait Self) "provide" (fun method =>
+      forall
+        (self : Ref.t Pointer.Kind.Ref Self)
+        (request : Ref.t Pointer.Kind.MutRef Request.t),
+      Run.Trait method [] [] [ φ self; φ request ] unit
+    ).
+
+  Class Run (Self : Set) `{Link Self} : Set := {
+    (* TODO: Add source *)
+    description : Run_description Self;
+    (* TODO: Add cause *)
+    provide : Run_provide Self;
+  }.
+End Error.
